src/asn1/ASN1.Low.BIT_STRING.fst
@@ -1,0 +1,146 @@
+module ASN1.Low.BIT_STRING
+
+open ASN1.Base
+open ASN1.Spec.BIT_STRING
+
+open ASN1.Low.Base
+open ASN1.Low.Tag
+open ASN1.Low.Length
+
+open LowParse.Low.Bytes
+
+open FStar.Integers
+
+module HS = FStar.HyperStack
+module HST = FStar.HyperStack.ST
+module MB = LowStar.Monotonic.Buffer
+module B = LowStar.Buffer
+module Cast = FStar.Int.Cast
+module B32 = FStar.Bytes
+
+// let encode_asn1_bit_string
+//   (len: asn1_int32_of_type BIT_STRING)
+//   (x: datatype_of_asn1_type BIT_STRING {
+//            let (|bits, s|) = x in
+//            let bytes_length = normalize_term ((bits + 7) / 8) in
+//            let unused_bits = normalize_term ((bytes_length * 8) - bits) in
+//            v len == bytes_length + 1 })
+// : Tot (ls: parse_filter_refine (filter_asn1_bit_string (v len)) { ls == synth_asn1_bit_string_inverse (v len) x })
+// = let (|bits, s|) = x in
+//   let bytes_len: len:asn1_int32 { v len <= asn1_length_max - 1 } = len - 1ul in
+//   let unused_bits: n:nat{0 <= n /\ n <= 7} = normalize_term ((v bytes_len * 8) - bits) in
+//   // assert (Seq.length s == bytes_length);
+//   let ls: parse_filter_refine (filter_asn1_bit_string (v len))
+//       = normalize_term (Seq.create 1 (u unused_bits) `Seq.append` s) in
+//   // assert_norm (bytes_length == 0 ==>
+//   //                unused_bits == 0);
+//   // assert_norm (bytes_length <> 0 ==>
+//   //                unused_bits <= 7 /\
+//   //               (bytes_length * 8 - unused_bits == bits));
+//   // assert (Seq.slice ls 1 l `Seq.equal` s);
+//   // assert (x == synth_asn1_bit_string l ls);
+//   ls
+
+// let encode_asn1_bit_string
+//   (l: asn1_length_of_type BIT_STRING)
+//   (value: datatype_of_asn1_type BIT_STRING {
+//           let (|len, unused_bits, s|) = value in
+//           l == v len })
+// : Tot (raw: parse_filter_refine (filter_asn1_bit_string l) { raw == synth_asn1_bit_string_inverse l value })
+// = let raw = B32.create 1ul ()
+
+//   let (|len, unused_bits, s32|) = value in
+//   let raw = cast unused_bits `Seq.cons` B32.reveal s32 in
+//   let (|len', unused_bits', s32'|) = synth_asn1_bit_string l raw in
+//   B32.extensionality s32 s32';
+//   raw
+
+#push-options "--query_stats --z3rlimit 32"
+let serialize32_asn1_bit_string_backwards
+  (len: asn1_int32_of_type BIT_STRING)
+: Tot (serializer32_backwards (serialize_asn1_bit_string (v len)))
+= fun (value: datatype_of_asn1_type BIT_STRING {
+            let (|len', unused_bits, s|) = value in
+            v len == v len' })
+    (#rrel #rel: _)
+    (b: B.mbuffer byte_t rrel rel)
+    (pos: size_t)
+->  (* Prf *) serialize_asn1_bit_string_unfold (v len) (value);
+    (* Prf *) let h0 = HST.get () in
+    let (|len, unused_bits, s32|) = value in
+    let leading_byte: byte = cast unused_bits in
+    (* Prf *) writable_weaken
+              (* buf *) b
+              (*range*) (v pos - v len) (v pos)
+              (* mem *) h0
+              (* from*) (v pos - v len)
+              (* to  *) (v pos - v len + 1);
+
+    mbuffer_upd (* <-- NOTE: Serializing the leading "unused_bits" byte. *)
+      (* buf *) b
+      (*range*) (v pos - v len) (v pos)
+      (* pos *) (pos - len)
+      (* val *) leading_byte;
+
+    (* Prf *) let h1 = HST.get () in
+    (* Prf *) writable_modifies
+              (* buf *) b
+              (*range*) (v pos - v len) (v pos)
+              (* mem *) h0
+              (*other*) B.loc_none
+              (* mem'*) h1;
+    (* Prf *) writable_weaken
+              (* buf *) b
+              (*range*) (v pos - v len) (v pos)
+              (* mem *) h1
+              (* from*) (v pos - v len + 1)
+              (* to  *) (v pos);
+
+    store_bytes (* <-- NOTE: Serializing the following bytes. *)
+      (* src *) s32
+      (*range*) 0ul (len - 1ul)
+      (* dst *) b
+      (* pos *) (pos - len + 1ul);
+
+    (* Prf *) let h2 = HST.get () in
+    (* Prf *) B.modifies_buffer_from_to_elim
+              (* buf *) b
+              (*frame*) (pos - len) (pos - len + 1ul)
+              (* new *) (B.loc_buffer_from_to b (pos - len + 1ul) pos)
+              (* mem *) h1
+              (* mem'*) h2;
+    (* Prf *) Seq.lemma_split (Seq.slice (B.as_seq h2 b) (v pos - v len) (v pos)) 1;
+(*return*) len
+
+let parser_tag_of_bit_string_impl
+  (x: datatype_of_asn1_type BIT_STRING)
+: Tot (tg: (the_asn1_type BIT_STRING & asn1_int32_of_type BIT_STRING) {
+           tg == parser_tag_of_bit_string x
+  })
+= let (|len, unused_bits, s32|) = x in
+  (BIT_STRING, len)
+
+let synth_asn1_bit_string_TLV_inverse_impl
+  (tag: (the_asn1_type BIT_STRING & asn1_int32_of_type BIT_STRING))
+  (value': refine_with_tag parser_tag_of_bit_string tag)
+: Tot (value: datatype_of_asn1_type BIT_STRING {
+                 let (|len, unused_bits, s|) = value in
+                 v (snd tag) == v len /\
+                 value == synth_asn1_bit_string_TLV_inverse tag value'})
+= value'
+
+let serialize32_asn1_bit_string_TLV_backwards ()
+: Tot (serializer32_backwards (serialize_asn1_bit_string_TLV))
+= serialize32_tagged_union_backwards
+  (* lst *) (serialize32_the_asn1_tag_backwards BIT_STRING
+             `serialize32_nondep_then_backwards`
+             serialize32_asn1_length_of_type_backwards BIT_STRING)
+  (* ltg *) (parser_tag_of_bit_string_impl)
+  (* ls  *) (fun parser_tag -> (serialize32_synth_backwards
+                              (* ls *) (weak_kind_of_type BIT_STRING
+                                        `serialize32_weaken_backwards`
+                                        serialize32_asn1_bit_string_backwards (snd parser_tag))
+                              (* f2 *) (synth_asn1_bit_string_TLV parser_tag)
+                              (* g1 *) (synth_asn1_bit_string_TLV_inverse parser_tag)
+                              (* g1'*) (synth_asn1_bit_string_TLV_inverse_impl parser_tag)
+                              (* prf*) ()))
