src/asn1/ASN1.Low.INTEGER.fst
@@ -44,226 +44,323 @@ NOTE: Since there are no low-level machine-integer to bytes implementations
 open LowParse.Low.BoundedInt
 
 #restart-solver
-#push-options "--query_stats --z3rlimit 32"
-let serialize32_asn1_integer
+#push-options "--query_stats --z3rlimit 512"
+let serialize32_asn1_integer_backwards
   (len: asn1_int32_of_type INTEGER)
-: Tot (serializer32 (serialize_asn1_integer (v len)))
+: Tot (serializer32_backwards (serialize_asn1_integer (v len)))
 = fun (value: datatype_of_asn1_type INTEGER { v len == length_of_asn1_integer value })
     (#rrel #rel: _)
     (b: B.mbuffer byte_t rrel rel)
     (pos: size_t)
-->(* 1-byte integer with the most-significant bit `0` *)
+->
+  (* NOTE: Using 1 byte to store a 1-byte integer with the most-significant bit `0` *)
   if      (0l         <= value && value <= 0x7Fl      ) then
-  ( admit (); (* Prf *) serialize_asn1_integer_unfold (length_of_asn1_integer value) value
+  ( (* Prf *) serialize_asn1_integer_unfold (length_of_asn1_integer value) value
   ; let b0: byte = cast #(Signed W32) #(Unsigned W8) value in
     (* Prf *) E.reveal_be_to_n (Seq.create 1 b0)
   ; (* Prf *) E.reveal_be_to_n (Seq.slice (Seq.create 1 b0) 1 1)
-  ; mbuffer_upd
-    (* dst *) (b)
-    (*range*) (v pos) (v pos + 1)
-    (* pos *) (pos)
-    (* val *) (b0)
+  ; mbuffer_upd (* <-- NOTE: Serializing the 1-byte integer. *)
+      (* dst *) b
+      (*range*) (v pos - 1) (v pos)
+      (* pos *) (pos - 1ul)
+      (* val *) b0
   ; (*return*) 1ul )
 
-  (* 1-byte integer with the most-significant bit `1` *)
+  (* NOTE: Using 2 bytes to store a 1-byte integer with the most-significant bit `1` *)
   else if (0x7Fl       < value && value <= 0xFFl      ) then
-  ( admit ()
-  ; (* Prf *) serialize_asn1_integer_unfold (length_of_asn1_integer value) value;
-    (* Prf *) let h0 = HST.get () in
+  ( (* Prf *) serialize_asn1_integer_unfold (length_of_asn1_integer value) value
+  ; (* Prf *) let h0 = HST.get () in
     (* Prf *) writable_weaken
-              (* buf *) (b)
-              (*range*) (v pos) (v pos + 2)
-              (* mem *) (h0)
-              (* from*) (v pos)
-              (* to  *) (v pos + 1);
-    (* NOTE: Serializing the leading zero. *)
-    mbuffer_upd
-      (* dst *) (b)
-      (*range*) (v pos) (v pos + 1)
-      (* pos *) (pos)
-      (* val *) (0x00uy);
-    (* Prf *) let h1 = HST.get () in
+              (* buf *) b
+              (*range*) (v pos - 2) (v pos)
+              (* mem *) h0
+              (* from*) (v pos - 2)
+              (* to  *) (v pos - 1)
+  ; mbuffer_upd (* <-- NOTE: Serializing the leading zero. *)
+      (* dst *) b
+      (*range*) (v pos - 2) (v pos - 1)
+      (* pos *) (pos - 2ul)
+      (* val *) 0x00uy
+  ; (* Prf *) let h1 = HST.get () in
     (* Prf *) writable_modifies
-              (* buf *) (b)
-              (*range*) (v pos) (v pos + 2)
-              (* mem *) (h0)
+              (* buf *) b
+              (*range*) (v pos - 2) (v pos)
+              (* mem *) h0
               (* loc *) (B.loc_none)
-              (* mem *) (h1);
-    (* Prf *) writable_weaken
-              (* buf *) (b)
-              (*range*) (v pos) (v pos + 2)
-              (* mem *) (h1)
-              (* from*) (v pos + 1)
-              (* to  *) (v pos + 2);
-    (* NOTE: Serializing the 1-byte integer. *)
-    let b0: byte = cast #(Signed W32) #(Unsigned W8) value in
-    (* Prf *) E.reveal_be_to_n (Seq.create 1 b0);
-    (* Prf *) E.reveal_be_to_n (Seq.slice (Seq.create 1 b0) 1 1);
-    mbuffer_upd
-      (* dst *) (b)
-      (*range*) (v pos) (v pos + 2)
-      (* pos *) (pos + 1ul)
-      (* val *) (b0);
-    (* Prf *) let h2 = HST.get () in
-    (* Prf *) Seq.lemma_split
-              (*slice*) (Seq.slice (B.as_seq h2 b) (v pos) (v pos + 2))
-              (* at  *) (1);
+              (* mem *) h1
+  ; (* Prf *) writable_weaken
+              (* buf *) b
+              (*range*) (v pos - 2) (v pos)
+              (* mem *) h1
+              (* from*) (v pos - 1)
+              (* to  *) (v pos)
+  ; let b0: byte = cast #(Signed W32) #(Unsigned W8) value in
+    (* Prf *) E.reveal_be_to_n (Seq.create 1 b0)
+  ; (* Prf *) E.reveal_be_to_n (Seq.slice (Seq.create 1 b0) 1 1)
+  ; mbuffer_upd (* <-- NOTE: Serializing the 1-byte integer. *)
+      (* dst *) b
+      (*range*) (v pos - 2) (v pos)
+      (* pos *) (pos - 1ul)
+      (* val *) b0
+  ; (* Prf *) let h2 = HST.get () in
     (* Prf *) B.modifies_buffer_from_to_elim
-              (* buf *) (b)
-              (*frame*) (pos) (pos + 1ul)
-              (* new *) (B.loc_buffer_from_to b (pos + 1ul) (pos + 2ul))
-              (* mem *) (h1) (h2);
-  (*return*) 2ul )
+              (* buf *) b
+              (*frame*) (pos - 2ul) (pos - 1ul)
+              (* new *) (B.loc_buffer_from_to b (pos - 1ul) (pos))
+              (* mem *) h1 h2
+  ; (* Prf *) Seq.lemma_split (Seq.slice (B.as_seq h2 b) (v pos - 2) (v pos)) 1
+  ; (*return*) 2ul )
 
-  (* 2-byte integer with the most-significant bit `0` *)
+  (* NOTE: Using 2 bytes to store a 2-byte integer with the most-significant bit `0` *)
   else if (0xFFl       < value && value <= 0x7FFFl    ) then
-  ( (* Prf *) serialize_asn1_integer_unfold (length_of_asn1_integer value) value;
-    (* Prf *) let h0 = HST.get () in
+  ( (* Prf *) serialize_asn1_integer_unfold (length_of_asn1_integer value) value
+  ; (* Prf *) let h0 = HST.get () in
     (* Prf *) LE.writable_store_pre
               (* buf *) b
-              (* from*) (v pos)
+              (* from*) (v pos - 2)
               (* len *) 2
               (*  p  *) (fun s -> E.be_to_n s == v #(Signed W32) value)
-              (* mem *) h0;
-    (* Prf *) let h1 = HST.get () in
-    LE.store16_be_i
+              (* mem *) h0
+  ; LE.store16_be_i  (* <-- NOTE: Serializing the 2-byte integer. *)
       (* buf *) b
-      (* pos *) pos
-      (* val *) (cast #(Signed W32) #(Unsigned W16) value);
+      (* pos *) (pos - 2ul)
+      (* val *) (cast #(Signed W32) #(Unsigned W16) value)
+  ; (* Prf *) let h1 = HST.get () in
     (* Prf *) LE.store_post_modifies
               (* buf *) b
-              (* from*) (v pos)
+              (* from*) (v pos - 2)
               (* len *) 2
-              (*  p  *) (fun s -> E.be_to_n s == v #(Signed W32) value);
-  (*return*) 2ul )
+              (*  p  *) (fun s -> E.be_to_n s == v #(Signed W32) value)
+              (* mem *) h0 h1
+  ; (*return*) 2ul )
 
-  (* 2-byte integer with the most-significant bit `1` *)
+  (* NOTE: Using 3 bytes to store a 2-byte integer with the most-significant bit `1` *)
   else if (0x7FFFl       < value && value <= 0xFFFFl    ) then
   ( (* Prf *) serialize_asn1_integer_unfold (length_of_asn1_integer value) value;
-    (* Prf *) serialize_bounded_integer_spec 2 (cast #(Signed W32) #(Unsigned W32) value);
-    let h0 = HST.get () in
-    writable_weaken b (v pos) (v pos + 3) h0 (v pos) (v pos + 1);
-    mbuffer_upd b (v pos) (v pos + 3) pos 0x00uy;
-    let h1 = HST.get () in
-    writable_modifies b (v pos) (v pos + 3) h0 B.loc_none h1;
-    writable_weaken b (v pos) (v pos + 3) h1 (v pos + 1) (v pos + 3);
-    let offset = serialize32_bounded_integer_2 () (cast #(Signed W32) #(Unsigned W32) value) b pos in
-    let h2 = HST.get () in
-    B.modifies_buffer_from_to_elim b pos (pos + 1ul) (B.loc_buffer_from_to b (pos + 1ul) (pos + 3ul)) h1 h2;
-  (*return*) 1ul + offset )
-  else admit ()
-
-
-(*)
-  (* NOTE: 3-byte integer with the most-significant bit `0` *)
-  else if (0xFFFFl      < value && value <= 0x7FFFFFl  ) then
-  ( (* Prf *) serialize_asn1_integer_unfold (length_of_asn1_integer value) value;
-    (* Prf *) assert_norm (v #(Signed W32) value < pow2 (8 * 3 - 1) /\
-                           v #(Signed W32) value < pow2 (8 * 3));
-    (* Prf *) E.reveal_n_to_be 3 (v #(Signed W32) value);
-    (* NOTE: Serialize the first and second bytes of this 3-byte integer. *)
-    let v01: uint_16 = cast #(Signed W32) #(Unsigned W16) (value / 0x100l) in
     (* Prf *) let h0 = HST.get () in
     (* Prf *) writable_weaken
-              (* buf *) (b)
-              (*range*) (v pos) (v pos + 3)
-              (* mem *) (h0)
-              (* from*) (v pos)
-              (* to  *) (v pos + 2);
-    (* Prf *) LE.writable_store_pre
-              (* dst *) (b)
-              (* from*) (v pos)
-              (* len *) (2)
-              (*predi*) (fun s -> E.be_to_n s == v v01)
-              (* mem *) (h0);
-    LE.store16_be_i
-    (* dst *) (b)
-    (* pos *) (pos)
-    (* val *) (v01);
+              (* buf *) b
+              (*range*) (v pos - 3) (v pos)
+              (* mem *) h0
+              (* from*) (v pos - 3)
+              (* to  *) (v pos - 2);
+    mbuffer_upd  (* <-- NOTE: Serializing the leading zero. *)
+      (* buf *) b
+      (*range*) (v pos - 3) (v pos)
+      (* pos *) (pos - 3ul)
+      (* val *) 0x00uy;
     (* Prf *) let h1 = HST.get () in
-    (* Prf *) LE.store_post_modifies
-              (* dst *) (b)
-              (* from*) (v pos)
-              (* len *) (2)
-              (*predi*) (fun s -> E.be_to_n s == v v01)
-              (* mem *) (h0)
-              (* mem'*) (h1);
-    (* NOTE: Serialize the third byte of this 3-byte integer. *)
-    let b2: byte = cast #(Signed W32) #(Unsigned W8) (value % 0x100l) in
-    (* Prf *) let h2 = HST.get () in
-    (* Prf *) E.reveal_be_to_n (Seq.create 1 b2);
-    (* Prf *) E.reveal_be_to_n (Seq.slice (Seq.create 1 b2) 1 1);
     (* Prf *) writable_modifies
-              (* buf *) (b)
-              (*range*) (v pos) (v pos + 3)
-              (* mem *) (h0)
-              (* loc *) (B.loc_none)
-              (* mem'*) (h1);
+              (* buf *) b
+              (*range*) (v pos - 3) (v pos)
+              (* mem *) h0
+              (*other*) B.loc_none
+              (* mem'*) h1;
     (* Prf *) writable_weaken
-              (* buf *) (b)
-              (*range*) (v pos) (v pos + 3)
-              (* mem *) (h1)
-              (* from*) (v pos + 2)
-              (* to  *) (v pos + 3);
-    mbuffer_upd
-    (* dst *) (b)
-    (*range*) (v pos) (v pos + 3)
-    (* pos *) (pos + 2ul)
-    (* val *) (b2);
-    (* Prf *) Seq.lemma_split
-              (*slice*) (Seq.slice (B.as_seq h2 b) (v pos) (v pos + 3))
-              (* at  *) (2);
+              (* buf *) b
+              (*range*) (v pos - 3) (v pos)
+              (* mem *) h1
+              (* from*) (v pos - 2)
+              (* to  *) (v pos);
+    (* Prf *) LE.writable_store_pre
+              (* buf *) b
+              (* from*) (v pos - 2)
+              (* len *) 2
+              (*  p  *) (fun s -> E.be_to_n s == v #(Signed W32) value)
+              (* mem *) h1;
+    LE.store16_be_i (* <-- NOTE: Serializing the 2-byte integer. *)
+      (* buf *) b
+      (* pos *) (pos - 2ul)
+      (* val *) (cast #(Signed W32) #(Unsigned W16) value);
+    (* Prf *) let h2 = HST.get () in
+    (* Prf *) LE.store_post_modifies
+              (* buf *) b
+              (* from*) (v pos - 2)
+              (* len *) 2
+              (*  p  *) (fun s -> E.be_to_n s == v #(Signed W32) value)
+              (* mem *) h1
+              (* mem'*) h2;
     (* Prf *) B.modifies_buffer_from_to_elim
-              (* buf *) (b)
-              (*frame*) (pos) (pos + 2ul)
-              (* new *) (B.loc_buffer_from_to b (pos + 2ul) (pos + 3ul))
-              (* mem *) (h1) (h2);
-  (*return*) 3ul )
+              (* buf *) b
+              (*frame*) (pos - 3ul) (pos - 2ul)
+              (* new *) (B.loc_buffer_from_to b (pos - 2ul) pos)
+              (* mem *) h1
+              (* mem'*) h2;
+    (* Prf *) Seq.lemma_split (Seq.slice (B.as_seq h2 b) (v pos - 3) (v pos)) 1;
+    (*return*) 3ul )
 
-  else (admit ())
+    (* Using 3 bytes to store a 3-byte integer with the most-significant bit `0` *)
+    else if (0xFFFFl      < value && value <= 0x7FFFFFl  ) then
+    ( (* Prf *) serialize_asn1_integer_unfold (length_of_asn1_integer value) value
+    ; assert_norm (v #(Signed W32) value < pow2 (8 * 3 - 1) /\
+                   v #(Signed W32) value < pow2 (8 * 3))
+    ; E.reveal_n_to_be 3 (v #(Signed W32) value)
+    ; let h0 = HST.get () in
+      (* Prf *) writable_weaken
+                (* buf *) b
+                (*range*) (v pos - 3) (v pos)
+                (* mem *) h0
+                (* from*) (v pos - 3)
+                (* to  *) (v pos - 1)
+    ; let first_2_bytes: uint_16 = cast #(Signed W32) #(Unsigned W16) (normalize_term (value / 0x100l)) in
+      (* Prf *) LE.writable_store_pre
+                (* buf *) b
+                (* from*) (v pos - 3)
+                (* len *) 2
+                (*  p  *) (fun s -> E.be_to_n s == v first_2_bytes)
+                (* mem *) h0
+    ; LE.store16_be_i
+        (* buf *) b
+        (* pos *) (pos - 3ul)
+        (* val *) first_2_bytes
+    ; let h1 = HST.get () in
+      (* Prf *) LE.store_post_modifies
+                (* buf *) b
+                (* from*) (v pos - 3)
+                (* len *) 2
+                (*  p  *) (fun s -> E.be_to_n s == v first_2_bytes)
+                (* mem *) h0
+                (* mem'*) h1
+    ; (* Prf *) writable_modifies
+                (* buf *) b
+                (*range*) (v pos - 3) (v pos)
+                (* mem *) h0
+                (*other*) B.loc_none
+                (* mem'*) h1
+    ; (* Prf *) writable_weaken
+                (* buf *) b
+                (*range*) (v pos - 3) (v pos)
+                (* mem *) h1
+                (* from*) (v pos - 1)
+                (* to  *) (v pos)
+    ; let last_byte: uint_8 = cast #(Signed W32) #(Unsigned W8) (normalize_term (value % 0x100l)) in
+      mbuffer_upd
+        (* buf *) b
+        (*range*) (v pos - 3) (v pos)
+        (* pos *) (pos - 1ul)
+        (* val *) last_byte
+    ; let h2 = HST.get () in
+      (* Prf *) B.modifies_buffer_from_to_elim
+              (* buf *) b
+              (*frame*) (pos - 3ul) (pos - 1ul)
+              (* new *) (B.loc_buffer_from_to b (pos - 1ul) pos)
+              (* mem *) h1
+              (* mem'*) h2
+    ; (* Prf *) Seq.lemma_split (Seq.slice (B.as_seq h2 b) (v pos - 3) (v pos)) 2
+    ; (*return*) 3ul )
 
-(*)
-  (* 2-byte integer with the mort-significant bit `0` *)
-  else if (0xFFl       < value && value <= 0x7FFFl    ) then
-  ( admit ();
-    (* Prf *) serialize_asn1_integer_unfold (length_of_asn1_integer value) value
-  ; (* Prf *) serialize_bounded_integer_spec 2 (cast #(Signed W32) #(Unsigned W32) value)
-  ; let offset = serialize32_bounded_integer_2 ()
-    (* val *) (cast #(Signed W32) #(Unsigned W32) value)
-    (* dst *) (b)
-    (* pos *) (pos) in
-  (*return*) offset )
+    (* Using 4 bytes to store a 3-byte integer with the most-significant bit `1` *)
+    else if (0x7FFFFFl      < value && value <= 0xFFFFFFl  ) then
+    ( (* Prf *) serialize_asn1_integer_unfold (length_of_asn1_integer value) value
+    ; assert_norm (v #(Signed W32) value < pow2 (8 * 3))
+    ; E.reveal_n_to_be 3 (v #(Signed W32) value)
+    ; let h0 = HST.get () in
+      (* Prf *) writable_weaken
+                (* buf *) b
+                (*range*) (v pos - 4) (v pos)
+                (* mem *) h0
+                (* from*) (v pos - 4)
+                (* to  *) (v pos - 3)
+    ; mbuffer_upd
+        (* buf *) b
+        (*range*) (v pos - 4) (v pos)
+        (* pos *) (pos - 4ul)
+        (* val *) 0x00uy
+    ; let h1 = HST.get () in
+      (* Prf *) writable_modifies
+                (* buf *) b
+                (*range*) (v pos - 4) (v pos)
+                (* mem *) h0
+                (*other*) B.loc_none
+                (* mem'*) h1
+    ; (* Prf *) writable_weaken
+                (* buf *) b
+                (*range*) (v pos - 4) (v pos)
+                (* mem *) h1
+                (* from*) (v pos - 3)
+                (* to  *) (v pos - 1)
+    ; let first_2_bytes: uint_16 = cast #(Signed W32) #(Unsigned W16) (normalize_term (value / 0x100l)) in
+      (* Prf *) LE.writable_store_pre
+                (* buf *) b
+                (* from*) (v pos - 3)
+                (* len *) 2
+                (*  p  *) (fun s -> E.be_to_n s == v first_2_bytes)
+                (* mem *) h1
+    ; LE.store16_be_i
+        (* buf *) b
+        (* pos *) (pos - 3ul)
+        (* val *) first_2_bytes
+    ; let h2 = HST.get () in
+      (* Prf *) LE.store_post_modifies
+                (* buf *) b
+                (* from*) (v pos - 3)
+                (* len *) 2
+                (*  p  *) (fun s -> E.be_to_n s == v first_2_bytes)
+                (* mem *) h1
+                (* mem'*) h2
+    ; (* Prf *) B.modifies_buffer_from_to_elim
+              (* buf *) b
+              (*frame*) (pos - 4ul) (pos - 3ul)
+              (* new *) (B.loc_buffer_from_to b (pos - 3ul) (pos - 1ul))
+              (* mem *) h1
+              (* mem'*) h2
+    ; (* Prf *) Seq.lemma_split (Seq.slice (B.as_seq h2 b) (v pos - 4) (v pos)) 1
+    ; (* Prf *) writable_modifies
+                (* buf *) b
+                (*range*) (v pos - 4) (v pos)
+                (* mem *) h1
+                (*other*) B.loc_none
+                (* mem'*) h2
+    ; (* Prf *) writable_weaken
+                (* buf *) b
+                (*range*) (v pos - 4) (v pos)
+                (* mem *) h2
+                (* from*) (v pos - 1)
+                (* to  *) (v pos)
+    ; let last_byte: uint_8 = cast #(Signed W32) #(Unsigned W8) (normalize_term (value % 0x100l)) in
+      mbuffer_upd
+        (* buf *) b
+        (*range*) (v pos - 4) (v pos)
+        (* pos *) (pos - 1ul)
+        (* val *) last_byte
+    ; let h3 = HST.get () in
+      (* Prf *) B.modifies_buffer_from_to_elim
+              (* buf *) b
+              (*frame*) (pos - 4ul) (pos - 1ul)
+              (* new *) (B.loc_buffer_from_to b (pos - 1ul) pos)
+              (* mem *) h2
+              (* mem'*) h3
+    ; (* Prf *) Seq.lemma_split (Seq.slice (B.as_seq h3 b) (v pos - 4) (v pos)) 1
+    ; (* Prf *) Seq.lemma_split (Seq.slice (B.as_seq h3 b) (v pos - 4) (v pos)) 3
+    ; (*return*) 4ul )
+
+  (* Using 4 bytes to store a 4-byte integer with the most-significant bit `0` *)
+  else if (0xFFFFFFl    < value && value <= 0x7FFFFFFFl) then
+  ( (* Prf *) serialize_asn1_integer_unfold (length_of_asn1_integer value) value
+  ; (* Prf *) assert_norm (v #(Signed W32) value < pow2 (8 * 4 - 1) /\
+                           v #(Signed W32) value < pow2 (8 * 4))
+  ; let value_of_all_4_bytes: uint_32 = (cast #(Signed W32) #(Unsigned W32) value) in
+    (* Prf *) let h0 = HST.get () in
+    (* Prf *) LE.writable_store_pre
+              (* buf *) b
+              (* from*) (v pos - 4)
+              (* len *) 4
+              (*  p  *) (fun s -> E.be_to_n s == v value_of_all_4_bytes)
+              (* mem *) h0
+  ; LE.store32_be_i
+      (* buf *) b
+      (* pos *) (pos - 4ul)
+      (* val *) value_of_all_4_bytes
+  ; (* Prf *) let h1 = HST.get () in
+    (* Prf *) LE.store_post_modifies
+              (* buf *) b
+              (* from*) (v pos - 4)
+              (* len *) 4
+              (*  p  *) (fun s -> E.be_to_n s == v value_of_all_4_bytes)
+              (* mem *) h0
+              (* mem'*) h1
+  ; (*return*) 4ul )
+
+  (* Unreachable *)
   else
-  ( admit () )
-#pop-options
-
-
-  // if      (0l         <= value && value <= 0x7Fl      ) then
-  // ( (* Prf *) serialize_asn1_integer_unfold (length_of_asn1_integer value) value
-  // ; let b0: byte = cast #(Signed W32) #(Unsigned W8) value in
-  //   (* Prf *) E.reveal_be_to_n (Seq.create 1 b0)
-  // ; (* Prf *) E.reveal_be_to_n (Seq.slice (Seq.create 1 b0) 1 1)
-  // ; mbuffer_upd
-  //   (* dst *) (b)
-  //   (*range*) (v pos) (v pos + 1)
-  //   (* pos *) (pos)
-  //   (* val *) (b0)
-  // ; (*return*) 1ul )
-
-  // (* 3-byte integer with the most-significant bit `1` *)
-  // else if (0x7FFFFFl     < value && value <= 0xFFFFFFl    ) then
-  // ( (* Prf *) serialize_asn1_integer_unfold (length_of_asn1_integer value) value
-  // ; let b0: byte = cast #(Signed W32) #(Unsigned W8) (value / 0x10000l) in
-  //   let v12: uint_16 = cast #(Signed W32) #(Unsigned W16) (value % 0x10000l) in
-  //   (* Prf *) E.reveal_be_to_n (Seq.create 1 b0)
-  // ; (* Prf *) E.reveal_be_to_n (Seq.slice (Seq.create 1 b0) 1 1)
-  // ; mbuffer_upd
-  //   (* dst *) (b)
-  //   (*range*) (v pos) (v pos + 1)
-  //   (* pos *) (pos)
-  //   (* val *) (b0)
-  // ; LE.store16_be_i
-  //   (* dst *) (b)
-  //   (* pos *) (pos + 1ul)
-  //   (* val *) (v12)
-  // ; (*return*) 3ul)
+  ( false_elim () )
