src/asn1/ASN1.Low.Length.fst
@@ -79,6 +79,26 @@ let serialize32_asn1_length_of_type
 = let min, max = asn1_length_min_of_type _a, asn1_length_max_of_type _a in
   LDER.serialize32_bounded_der_length32 min max
 
+// #push-options "--z3rlimit 16"
+// let offset_of_asn1_length_of_type_impl
+//   (_a: asn1_type)
+//   (len: asn1_int32_of_type _a)
+// : Tot (offset: size_t{v offset == Seq.length (serialize (serialize_asn1_length_of_type _a) len)})
+// = serialize_asn1_length_unfold len;
+//   serialize_asn1_length_of_type_eq _a len;
+//   let x = SDER.tag_of_der_length32_impl len in
+//   if x < 128uy then
+//   ( 1ul )
+//   else if x = 129uy then
+//   ( 2ul )
+//   else if x = 130uy then
+//   ( 3ul )
+//   else if x = 131uy then
+//   ( 4ul )
+//   else
+//   ( 5ul )
+// #pop-options
+
 let serialize32_asn1_length_of_type_backwards
   (_a: asn1_type)
 : Tot (serializer32_backwards (serialize_asn1_length_of_type _a))
@@ -86,7 +106,9 @@ let serialize32_asn1_length_of_type_backwards
     (#rrel #rel: _)
     (b: B.mbuffer byte_t rrel rel)
     (pos: size_t)
--> let offset = offset_of_asn1_length_impl len in
+-> (* Prf *) serialize_asn1_length_of_type_eq _a len;
+   (* Prf *) serialize_asn1_length_unfold len;
+   let offset = offset_of_asn1_length_impl len in
    (* Prf *) let h0 = HST.get () in
    let offset = serialize32_asn1_length_of_type _a len b (pos - offset) in
    (* Prf *) let h1 = HST.get () in
