src/asn1/ASN1.Spec.BIT_STRING.fst
@@ -1,0 +1,353 @@
+module ASN1.Spec.BIT_STRING
+
+open LowParse.Spec.Base
+open LowParse.Spec.Combinators
+open LowParse.Spec.SeqBytes.Base
+
+open ASN1.Base
+open ASN1.Spec.Tag
+open ASN1.Spec.Length
+
+open FStar.Integers
+
+module B32 = FStar.Bytes
+
+/// TEST
+///
+
+// let bs_empty   : datatype_of_asn1_type BIT_STRING = (|1ul, 0ul, B32.empty_bytes |)
+// let bs_0_unused: datatype_of_asn1_type BIT_STRING = (|2ul, 0ul, B32.create 1ul 0b1uy|)
+// let bs_1_unused: datatype_of_asn1_type BIT_STRING = (|2ul, 1ul, B32.create 1ul 0b10uy|)
+// let bs_2_unused: datatype_of_asn1_type BIT_STRING = (|2ul, 2ul, B32.create 1ul 0b100uy|)
+// let bs_3_unused: datatype_of_asn1_type BIT_STRING = (|2ul, 3ul, B32.create 1ul 0b1000uy|)
+// let bs_4_unused: datatype_of_asn1_type BIT_STRING = (|2ul, 4ul, B32.create 1ul 0b10000uy|)
+// let bs_5_unused: datatype_of_asn1_type BIT_STRING = (|2ul, 5ul, B32.create 1ul 0b100000uy|)
+// let bs_6_unused: datatype_of_asn1_type BIT_STRING = (|2ul, 6ul, B32.create 1ul 0b1000000uy|)
+// let bs_7_unused: datatype_of_asn1_type BIT_STRING = (|2ul, 7ul, B32.create 1ul 0b10000000uy|)
+
+(*
+   Len = 1, unused = 0, bytes = []
+   Len = 2, unused = x, bytes = [_]
+*)
+
+// let (.[]) = B32.index
+
+let filter_asn1_bit_string
+  (l: asn1_length_of_type BIT_STRING)
+  (raw: lbytes l)
+: GTot (bool)
+= let unused_bits = raw.[0] in
+  if l = 1 then
+  ( unused_bits = 0uy )
+  else
+  ( let mask = normalize_term (pow2 (v unused_bits)) in
+    0uy <= unused_bits && unused_bits <= 7uy &&
+    0 = normalize_term ((v raw.[l - 1]) % mask) )
+
+let synth_asn1_bit_string
+  (l: asn1_length_of_type BIT_STRING)
+  (raw: parse_filter_refine (filter_asn1_bit_string l))
+: GTot (value: datatype_of_asn1_type BIT_STRING {
+               let (|len, unused_bits, s|) = value in
+               l == v len })
+= let unused_bits: n: asn1_int32 {0 <= v n /\ v n <= 7} = cast raw.[0] in
+  let s32 = B32.hide (Seq.slice raw 1 l) in
+  (|u l, unused_bits, s32|)
+
+// let unused_bits = ls.[0] in
+//   let s = Seq.slice ls 1 l in
+//   if l = 1 then
+//   ( assert_norm ( v unused_bits == 0 )
+//   ; let bits: n:uint_32{v n == 0} = normalize_term (u ((l - 1) * 8 - (v unused_bits))) in
+//     (|bits, s|) )
+//   else
+//   ( assert_norm ( v unused_bits <= 7 )
+//   ; let bits: n:uint_32 {
+//         0 <= v n /\
+//         v n <= normalize_term (u ((asn1_length_max - 1) * 8))
+//     } = normalize_term (u ((l - 1) * 8 - (v unused_bits))) in
+//     (|bits, s|) )
+
+#push-options "--query_stats --z3rlimit 16"
+let synth_asn1_bit_string_injective'
+  (l: asn1_length_of_type BIT_STRING)
+  (raw1 raw2: parse_filter_refine (filter_asn1_bit_string l))
+: Lemma
+  (requires synth_asn1_bit_string l raw1 == synth_asn1_bit_string l raw2)
+  (ensures raw1 == raw2)
+= Seq.lemma_split raw1 1;
+  Seq.lemma_split raw2 1;
+  assert (raw1 `Seq.equal` raw2)
+  // let unused_bits1 = raw1.[0] in
+  // let unused_bits2 = raw2.[0] in
+  // let s1 = Seq.slice raw1 1 l in
+  // let s2 = Seq.slice raw2 1 l in
+  // assert ( unused_bits1 == unused_bits2 /\
+  //          s1 `Seq.equal` s2 /\
+  //          (unused_bits1 `Seq.cons` s1) `Seq.equal` raw1 /\
+  //          (unused_bits2 `Seq.cons` s2) `Seq.equal` raw2 );
+  // assert_norm ((unused_bits1 `Seq.cons` s1) `Seq.equal` raw1);
+  // assert_norm ((unused_bits2 `Seq.cons` s2) `Seq.equal` raw2);
+  // if l = 1 then
+  // ( assert_norm (unused_bits1 == unused_bits2) )
+
+  // ( let bits1: n:nat {
+  //       0 <= n /\
+  //       n <= normalize_term ((asn1_length_max - 1) * 8)
+  //   } = normalize_term ((l - 1) * 8 - (v unused_bits1)) in
+  //   let bits2: n:nat {
+  //       0 <= n /\
+  //       n <= normalize_term ((asn1_length_max - 1) * 8)
+  //   } = normalize_term ((l - 1) * 8 - (v unused_bits2)) in
+  //   assert_norm (bits1 == bits2)
+  // ; assert_norm (unused_bits1 == unused_bits2)
+  // ; assert_norm (s1 `Seq.equal` s2)
+  // ; assert_norm ((unused_bits1 `Seq.cons` s1) `Seq.equal` raw1)
+  // ; assert_norm ((unused_bits2 `Seq.cons` s2) `Seq.equal` raw2) )
+#pop-options
+
+let synth_asn1_bit_string_injective
+  (l: asn1_length_of_type BIT_STRING)
+: Lemma (
+  synth_injective (synth_asn1_bit_string l)
+)
+= synth_injective_intro'
+  (* f *) (synth_asn1_bit_string l)
+  (*prf*) (synth_asn1_bit_string_injective' l)
+
+let synth_asn1_bit_string_inverse
+  (l: asn1_length_of_type BIT_STRING)
+  (value: datatype_of_asn1_type BIT_STRING {
+          let (|len, unused_bits, s|) = value in
+          l == v len })
+: GTot (raw: parse_filter_refine (filter_asn1_bit_string l) { value == synth_asn1_bit_string l raw })
+= let (|len, unused_bits, s32|) = value in
+  let raw = cast unused_bits `Seq.cons` B32.reveal s32 in
+  let (|len', unused_bits', s32'|) = synth_asn1_bit_string l raw in
+  B32.extensionality s32 s32';
+  raw
+
+let parse_asn1_bit_string_kind (l: asn1_length_of_type BIT_STRING) = constant_size_parser_kind l
+let parse_asn1_bit_string
+  (l: asn1_length_of_type BIT_STRING)
+: parser (parse_asn1_bit_string_kind l)
+         (value: datatype_of_asn1_type BIT_STRING {
+                 let (|len, unused_bits, s|) = value in
+                 l == v len })
+= synth_asn1_bit_string_injective l;
+  parse_seq_flbytes l
+  `parse_filter`
+  filter_asn1_bit_string l
+  `parse_synth`
+  synth_asn1_bit_string l
+
+let parse_asn1_bit_string_unfold
+  (l: asn1_length_of_type BIT_STRING)
+  (input: bytes)
+: Lemma (
+  parse (parse_asn1_bit_string l) input ==
+ (match parse (parse_seq_flbytes l) input with
+  | None -> None
+  | Some (raw, consumed) -> ( if filter_asn1_bit_string l raw then
+                              ( Some (synth_asn1_bit_string l raw, consumed) )
+                              else
+                              ( None )) )
+)
+= parser_kind_prop_equiv (get_parser_kind (parse_seq_flbytes l)) (parse_seq_flbytes l);
+  parser_kind_prop_equiv (get_parser_kind (parse_asn1_bit_string l)) (parse_asn1_bit_string l);
+  parse_filter_eq
+  (* p *) (parse_seq_flbytes l)
+  (* f *) (filter_asn1_bit_string l)
+  (* in*) (input);
+  synth_asn1_bit_string_injective l;
+  parse_synth_eq
+  (* p *) (parse_seq_flbytes l
+           `parse_filter`
+           filter_asn1_bit_string l)
+  (* f *) (synth_asn1_bit_string l)
+  (* in*) (input)
+
+let serialize_asn1_bit_string
+  (l: asn1_length_of_type BIT_STRING)
+: serializer (parse_asn1_bit_string l)
+= serialize_synth
+  (* p1 *) (parse_seq_flbytes l
+            `parse_filter`
+            filter_asn1_bit_string l)
+  (* f2 *) (synth_asn1_bit_string l)
+  (* s1 *) (serialize_seq_flbytes l
+            `serialize_filter`
+            filter_asn1_bit_string l)
+  (* g1 *) (synth_asn1_bit_string_inverse l)
+  (* prf*) (synth_asn1_bit_string_injective l)
+
+let serialize_asn1_bit_string_unfold
+  (l: asn1_length_of_type BIT_STRING)
+  (value: datatype_of_asn1_type BIT_STRING {
+                 let (|len, unused_bits, s|) = value in
+                 l == v len })
+: Lemma (
+  serialize (serialize_asn1_bit_string l) value ==
+  serialize (serialize_seq_flbytes l) (synth_asn1_bit_string_inverse l value))
+= serialize_synth_eq
+  (* p1 *) (parse_seq_flbytes l
+            `parse_filter`
+            filter_asn1_bit_string l)
+  (* f2 *) (synth_asn1_bit_string l)
+  (* s1 *) (serialize_seq_flbytes l
+            `serialize_filter`
+            filter_asn1_bit_string l)
+  (* g1 *) (synth_asn1_bit_string_inverse l)
+  (* prf*) (synth_asn1_bit_string_injective l)
+  (* val*) (value)
+
+
+////////// TLV //////////
+let parser_tag_of_bit_string
+  (x: datatype_of_asn1_type BIT_STRING)
+: GTot (the_asn1_type BIT_STRING & asn1_int32_of_type BIT_STRING)
+= let (|len, unused_bits, s32|) = x in
+  (BIT_STRING, len)
+
+let synth_asn1_bit_string_TLV
+  (tag: (the_asn1_type BIT_STRING & asn1_int32_of_type BIT_STRING))
+  (value: datatype_of_asn1_type BIT_STRING {
+                 let (|len, unused_bits, s|) = value in
+                 v (snd tag) == v len })
+: GTot (value': refine_with_tag parser_tag_of_bit_string tag)
+= value
+
+let synth_asn1_bit_string_TLV_inverse
+  (tag: (the_asn1_type BIT_STRING & asn1_int32_of_type BIT_STRING))
+  (value': refine_with_tag parser_tag_of_bit_string tag)
+: GTot (value: datatype_of_asn1_type BIT_STRING {
+                 let (|len, unused_bits, s|) = value in
+                 v (snd tag) == v len /\
+                 value' == synth_asn1_bit_string_TLV tag value})
+= value'
+
+let parse_asn1_bit_string_TLV_kind
+: parser_kind
+= parse_asn1_tag_kind
+  `and_then_kind`
+  parse_asn1_length_kind_of_type BIT_STRING
+  `and_then_kind`
+  weak_kind_of_type BIT_STRING
+
+let parse_asn1_bit_string_TLV
+: parser parse_asn1_bit_string_TLV_kind (datatype_of_asn1_type BIT_STRING)
+= parse_tagged_union
+  (* pt *) (parse_the_asn1_tag BIT_STRING
+            `nondep_then`
+            parse_asn1_length_of_type BIT_STRING)
+  (* tg *) (parser_tag_of_bit_string)
+  (* p  *) (fun parser_tag -> weak_kind_of_type BIT_STRING
+                            `weaken`
+                           (parse_asn1_bit_string (v (snd parser_tag))
+                            `parse_synth`
+                            synth_asn1_bit_string_TLV parser_tag))
+
+#push-options "--query_stats --z3rlimit 32"
+let parse_asn1_bit_string_TLV_unfold
+  (input: bytes)
+: Lemma (
+  parse parse_asn1_bit_string_TLV input ==
+ (match parse (parse_the_asn1_tag BIT_STRING) input with
+  | None -> None
+  | Some (tag, consumed_tag) ->
+    (let input_LV = Seq.slice input consumed_tag (Seq.length input) in
+     match parse (parse_asn1_length_of_type BIT_STRING) input_LV with
+     | None -> None
+     | Some (len, consumed_len) ->
+       (let input_V = Seq.slice input_LV consumed_len (Seq.length input_LV) in
+        match parse (parse_asn1_bit_string (v len)) input_V with
+        | None -> None
+        | Some (value, consumed_value) ->
+               Some ((synth_asn1_bit_string_TLV (tag, len) value),
+                     (consumed_tag + consumed_len + consumed_value <: consumed_length input)))))
+)
+= parser_kind_prop_equiv (get_parser_kind (parse_the_asn1_tag BIT_STRING)) (parse_the_asn1_tag BIT_STRING);
+  parser_kind_prop_equiv (get_parser_kind (parse_asn1_length_of_type BIT_STRING)) (parse_asn1_length_of_type BIT_STRING);
+
+  nondep_then_eq
+  (* p1 *) (parse_the_asn1_tag BIT_STRING)
+  (* p2 *) (parse_asn1_length_of_type BIT_STRING)
+  (* in *) (input);
+
+  let parser_tag = (parse_the_asn1_tag BIT_STRING
+                    `nondep_then`
+                    parse_asn1_length_of_type BIT_STRING) input in
+  if Some? parser_tag then
+  ( let Some (parser_tag, length) = parser_tag in
+    parser_kind_prop_equiv (get_parser_kind (parse_asn1_bit_string length)) (parse_asn1_bit_string length);
+    parse_synth_eq
+    (* p *) (parse_asn1_bit_string (v (snd parser_tag)))
+    (* f *) (synth_asn1_bit_string_TLV parser_tag)
+    (* in*) (Seq.slice input length (Seq.length input)) );
+
+  parse_tagged_union_eq
+  (* pt *) (parse_the_asn1_tag BIT_STRING
+            `nondep_then`
+            parse_asn1_length_of_type BIT_STRING)
+  (* tg *) (parser_tag_of_bit_string)
+  (* p  *) (fun parser_tag -> weak_kind_of_type BIT_STRING
+                            `weaken`
+                           (parse_asn1_bit_string (v (snd parser_tag))
+                            `parse_synth`
+                            synth_asn1_bit_string_TLV parser_tag))
+  (* in *) (input);
+
+(*FIXME:*) admit()
+#pop-options
+
+#push-options "--query_stats --initial_fuel 4"
+let serialize_asn1_bit_string_TLV
+: serializer parse_asn1_bit_string_TLV
+= serialize_tagged_union
+  (* st *) (serialize_the_asn1_tag BIT_STRING
+            `serialize_nondep_then`
+            serialize_asn1_length_of_type BIT_STRING)
+  (* tg *) (parser_tag_of_bit_string)
+  (* s  *) (fun parser_tag -> weak_kind_of_type BIT_STRING
+                            `serialize_weaken`
+                           (serialize_synth
+                            (* p1 *) (parse_asn1_bit_string (v (snd parser_tag)))
+                            (* f2 *) (synth_asn1_bit_string_TLV parser_tag)
+                            (* s1 *) (serialize_asn1_bit_string (v (snd parser_tag)))
+                            (* g1 *) (synth_asn1_bit_string_TLV_inverse parser_tag)
+                            (* prf*) ()))
+#pop-options
+
+(*)
+#push-options "--query_stats --z3rlimit 32"
+let serialize_asn1_bit_string_TLV_unfold
+  (value: datatype_of_asn1_type BIT_STRING)
+: Lemma (
+  serialize serialize_asn1_bit_string_TLV value ==
+  serialize (serialize_the_asn1_tag BIT_STRING) BIT_STRING
+  `Seq.append`
+  serialize (serialize_asn1_length_of_type BIT_STRING) (dfst value)
+  `Seq.append`
+  serialize (serialize_asn1_bit_string (v (dfst value))) value
+)
+= serialize_nondep_then_eq
+  (* s1 *) (serialize_the_asn1_tag BIT_STRING)
+  (* s2 *) (serialize_asn1_length_of_type BIT_STRING)
+  (* in *) (parser_tag_of_bit_string value);
+  serialize_asn1_bit_string_unfold (parser_tag_of_bit_string value) value;
+  serialize_tagged_union_eq
+  (* st *) (serialize_the_asn1_tag BIT_STRING
+            `serialize_nondep_then`
+            serialize_asn1_length_of_type BIT_STRING)
+  (* tg *) (parser_tag_of_bit_string)
+  (* s  *) (fun parser_tag -> weak_kind_of_type BIT_STRING
+                            `serialize_weaken`
+                           (serialize_synth
+                            (* p1 *) (parse_asn1_bit_string (v (snd parser_tag)))
+                            (* f2 *) (synth_asn1_bit_string_TLV parser_tag)
+                            (* s1 *) (serialize_asn1_bit_string (v (snd parser_tag)))
+                            (* g1 *) (synth_asn1_bit_string_TLV_inverse parser_tag)
+                            (* prf*) ()))
+  (* in *) (value)
+#pop-options
+
