src/asn1/ASN1.Spec.Length.fst
@@ -23,6 +23,7 @@ let serialize_asn1_length
 
 let serialize_asn1_length_unfold = serialize_bounded_der_length32_unfold asn1_length_min asn1_length_max
 
+
 #push-options "--z3rlimit 16"
 let len_of_asn1_length
   (len: asn1_int32)
@@ -55,15 +56,13 @@ let len_of_asn1_length
 let parse_asn1_length_kind_of_type
   (_a: asn1_type)
 : parser_kind
-= let min, max = asn1_length_min_of_type _a, asn1_length_max_of_type _a in
-  parse_bounded_der_length32_kind min max
+= parse_bounded_der_length32_kind (asn1_length_min_of_type _a) (asn1_length_max_of_type _a)
 
 let parse_asn1_length_of_type
   (_a: asn1_type)
 // : parser parse_asn1_length_kind (parse_filter_refine (filter_asn1_length_of_type _a))
 : parser (parse_asn1_length_kind_of_type _a) (asn1_int32_of_type _a)
-= let min, max = asn1_length_min_of_type _a, asn1_length_max_of_type _a in
-  parse_bounded_der_length32 min max
+= parse_bounded_der_length32 (asn1_length_min_of_type _a) (asn1_length_max_of_type _a)
   // parse_asn1_length
   // `parse_filter`
   // filter_asn1_length_of_type _a
@@ -71,20 +70,55 @@ let parse_asn1_length_of_type
 let parse_asn1_length_of_type_unfold
   (_a: asn1_type)
   (input: bytes)
-= let min, max = asn1_length_min_of_type _a, asn1_length_max_of_type _a in
-  parse_bounded_der_length32_unfold min max input
+= parse_bounded_der_length32_unfold (asn1_length_min_of_type _a) (asn1_length_max_of_type _a) input
 
+unfold
 let serialize_asn1_length_of_type
   (_a: asn1_type)
 : serializer (parse_asn1_length_of_type _a)
-= let min, max = asn1_length_min_of_type _a, asn1_length_max_of_type _a in
-  serialize_bounded_der_length32 min max
+= serialize_bounded_der_length32 (asn1_length_min_of_type _a) (asn1_length_max_of_type _a)
 // = serialize_asn1_length
 //   `serialize_filter`
 //   filter_asn1_length_of_type _a
 
-let serialize_asn1_length_of_type_unfold
+// let serialize_asn1_length_of_type_unfold
+//   (_a: asn1_type)
+//   (len: asn1_int32_of_type _a)
+// = serialize_bounded_der_length32_unfold (asn1_length_min_of_type _a) (asn1_length_max_of_type _a) len
+
+// let serialize_asn1_length_of_type_size
+//   (_a: asn1_type)
+//   (len: asn1_int32_of_type _a)
+// = serialize_bounded_der_length32_size (asn1_length_min_of_type _a) (asn1_length_max_of_type _a) len
+
+let serialize_asn1_length_of_type_eq
   (_a: asn1_type)
   (len: asn1_int32_of_type _a)
-= let min, max = asn1_length_min_of_type _a, asn1_length_max_of_type _a in
+: Lemma (
+  serialize serialize_asn1_length len ==
+  serialize (serialize_asn1_length_of_type _a) len
+)
+= serialize_asn1_length_unfold len;
+  let min, max = asn1_length_min_of_type _a, asn1_length_max_of_type _a in
   serialize_bounded_der_length32_unfold min max len
+
+// #push-options "--z3rlimit 16"
+// let len_of_asn1_length_of_type
+//   (_a: asn1_type)
+//   (len: asn1_int32_of_type _a)
+// : Tot (offset: uint_32{v offset == Seq.length (serialize (serialize_asn1_length_of_type _a) len)})
+// = serialize_asn1_length_unfold len;
+//   serialize_asn1_length_of_type_eq _a len;
+//   let x = tag_of_der_length32_impl len in
+//   if x < 128uy then
+//   ( 1ul )
+//   else if x = 129uy then
+//   ( 2ul )
+//   else if x = 130uy then
+//   ( 3ul )
+//   else if x = 131uy then
+//   ( 4ul )
+//   else
+//   ( 5ul )
+// #pop-options
+
