src/asn1/RIoT.Test.fst
@@ -1,0 +1,23 @@
+module RIoT.Test
+
+open LowParse.Low.Base
+open LowParse.Low.Combinators
+
+open ASN1.Spec
+open ASN1.Low
+
+module U8 = FStar.UInt8
+module U32 = FStar.UInt32
+module HS = FStar.HyperStack
+module HST = FStar.HyperStack.ST
+module MB = LowStar.Monotonic.Buffer
+module B = LowStar.Buffer
+module Cast = FStar.Int.Cast
+module C = C
+
+open FStar.Integers
+
+let main ()
+: HST.St C.exit_code
+= C.EXIT_SUCCESS
+
